Checkpoint, working towards UndefRefinementFacts.v...

src/coq/Handlers/Pick.v
@@ -45,7 +45,9 @@ Import MonadNotation.
   - The executable one interprets [undef] as 0 at the type
 *)
 
-Module Make(A:MemoryAddress.ADDRESS)(SIZEOF: Sizeof)(LLVMIO: LLVM_INTERACTIONS(A)(SIZEOF))(PTOI:PTOI(A))(PROVENANCE:PROVENANCE(A))(ITOP:ITOP(A)(PROVENANCE))(GEP:GEPM(A)(SIZEOF)(LLVMIO))(BYTE_IMPL : ByteImpl(A)(SIZEOF)(LLVMIO))(Conc : Concretize A SIZEOF LLVMIO).
+Module Make(A:MemoryAddress.ADDRESS)(SIZEOF: Sizeof)(LLVMIO: LLVM_INTERACTIONS(A)(SIZEOF))(PTOI:PTOI(A))(PROVENANCE:PROVENANCE(A))(ITOP:ITOP(A)(PROVENANCE))(GEP:GEPM(A)(SIZEOF)(LLVMIO))(BYTE_IMPL : ByteImpl(A)(SIZEOF)(LLVMIO)).
+
+  Module Conc := Serialization.Make A SIZEOF LLVMIO PTOI PROVENANCE ITOP GEP BYTE_IMPL.
   Import Conc.
   Import LLVMIO.
 
@@ -76,219 +78,14 @@ Module Make(A:MemoryAddress.ADDRESS)(SIZEOF: Sizeof)(LLVMIO: LLVM_INTERACTIONS(A
 
     Open Scope N_scope.
 
-    Definition default_dvalue_of_dtyp_i (sz : N) : err dvalue:=
-       (if (sz =? 64) then ret (DVALUE_I64 (repr 0))
-        else if (sz =? 32) then ret (DVALUE_I32 (repr 0))
-            else if (sz =? 8) then ret (DVALUE_I8 (repr 0))
-                  else if (sz =? 1) then ret (DVALUE_I1 (repr 0))
-                       else failwith
-              "Illegal size for generating default dvalue of DTYPE_I").
-
-
-    (* Handler for PickE which concretizes everything to 0 *)
-    Fixpoint default_dvalue_of_dtyp (dt : dtyp) : err dvalue :=
-      match dt with
-      | DTYPE_I sz => default_dvalue_of_dtyp_i sz
-      | DTYPE_IPTR => ret (DVALUE_IPTR 0)
-      | DTYPE_Pointer => ret (DVALUE_Addr A.null)
-      | DTYPE_Void => ret DVALUE_None
-      | DTYPE_Half => failwith "Unimplemented default type: half"
-      | DTYPE_Float => ret (DVALUE_Float Float32.zero)
-      | DTYPE_Double => ret (DVALUE_Double (Float32.to_double Float32.zero))
-      | DTYPE_X86_fp80 => failwith "Unimplemented default type: x86_fp80"
-      | DTYPE_Fp128 => failwith "Unimplemented default type: fp128"
-      | DTYPE_Ppc_fp128 => failwith "Unimplemented default type: ppc_fp128"
-      | DTYPE_Metadata => failwith "Unimplemented default type: metadata"
-      | DTYPE_X86_mmx => failwith "Unimplemented default type: x86_mmx"
-      | DTYPE_Opaque => failwith "Unimplemented default type: opaque"
-      | DTYPE_Array sz t =>
-        if (0 <=? sz) then
-          v <- default_dvalue_of_dtyp t ;;
-          (ret (DVALUE_Array (repeat v (N.to_nat sz))))
-        else
-          failwith ("Negative array length for generating default value" ++
-          "of DTYPE_Array or DTYPE_Vector")
-
-      (* Matching valid Vector types... *)
-      (* Currently commented out unsupported ones *)
-      (* | DTYPE_Vector sz (DTYPE_Half) => *)
-      (*   if (0 <=? sz) then *)
-      (*     (ret (DVALUE_Vector *)
-      (*             (repeat (DVALUE_Float Float32.zero) (N.to_nat sz)))) *)
-      (*   else *)
-      (*     failwith ("Negative array length for generating default value" ++ *)
-      (*     "of DTYPE_Array or DTYPE_Vector") *)
-      | DTYPE_Vector sz (DTYPE_Float) =>
-        if (0 <=? sz) then
-          (ret (DVALUE_Vector
-                  (repeat (DVALUE_Float Float32.zero) (N.to_nat sz))))
-        else
-          failwith ("Negative array length for generating default value" ++
-          "of DTYPE_Array or DTYPE_Vector")
-      | DTYPE_Vector sz (DTYPE_Double) =>
-        if (0 <=? sz) then
-          (ret (DVALUE_Vector
-                  (repeat (DVALUE_Double (Float32.to_double Float32.zero))
-                          (N.to_nat sz))))
-        else
-          failwith ("Negative array length for generating default value" ++
-          "of DTYPE_Array or DTYPE_Vector")
-      (* | DTYPE_Vector sz (DTYPE_X86_fp80) => *)
-      (*   if (0 <=? sz) then *)
-      (*     (ret (DVALUE_Vector *)
-      (*             (repeat (DVALUE_Float Float32.zero) (N.to_nat sz)))) *)
-      (*   else *)
-      (*     failwith ("Negative array length for generating default value" ++ *)
-      (*     "of DTYPE_Array or DTYPE_Vector") *)
-      (* | DTYPE_Vector sz (DTYPE_Fp128) => *)
-      (*   if (0 <=? sz) then *)
-      (*     (ret (DVALUE_Vector *)
-      (*             (repeat (DVALUE_Float Float32.zero) (N.to_nat sz)))) *)
-      (*   else *)
-      (*     failwith ("Negative array length for generating default value" ++ *)
-      (*     "of DTYPE_Array or DTYPE_Vector") *)
-      | DTYPE_Vector sz (DTYPE_I n) =>
-        if (0 <=? sz) then
-          v <- default_dvalue_of_dtyp_i n ;;
-          (ret (DVALUE_Vector (repeat v (N.to_nat sz))))
-        else
-          failwith ("Negative array length for generating default value" ++
-          "of DTYPE_Array or DTYPE_Vector")
-      | DTYPE_Vector _ _ => failwith ("Non-valid vector type when" ++
-          "generating default vector")
-      | DTYPE_Struct fields =>
-        v <- @map_monad err _ dtyp dvalue default_dvalue_of_dtyp fields;;
-        ret (DVALUE_Struct v)
-      | DTYPE_Packed_struct fields =>
-        v <- @map_monad err _ dtyp dvalue default_dvalue_of_dtyp fields;;
-        ret (DVALUE_Packed_struct v)
-      end.
-
     Import MonadNotation.
-
-    Ltac do_it := constructor; cbn; auto; fail.
-
-    Lemma forall_repeat_true:
-      forall A (f : A -> Prop) n x, f x -> Forall (fun y : A => f y) (repeat x n).
-    Proof.
-      intros. induction n. cbn. constructor.
-      constructor. auto. cbn. apply IHn.
-    Qed.
-
-    Lemma dvalue_default : forall t v,
-        inr v = (default_dvalue_of_dtyp t) ->
-        dvalue_has_dtyp v t.
-    Proof.
-      intros t v. revert v.
-      induction t; try do_it;
-        try (intros; subst; inversion H; constructor).
-      - intros. subst. cbn in H.
-        unfold default_dvalue_of_dtyp_i in H.
-        destruct (@IX_supported_dec a).
-        * inversion i; subst; cbn in H; inversion H; constructor; auto.
-        * rewrite unsupported_cases in H; auto. inversion H.
-      - intros. subst. inversion H. clear H.
-        induction sz.
-        + cbn in H1.
-          destruct (default_dvalue_of_dtyp t) eqn: HT. inv H1. inv H1.
-          pose proof DVALUE_Array_typ.
-          specialize (H nil (N.to_nat 0) t).
-          rewrite Nnat.N2Nat.id in H.
-          apply H. auto. auto.
-        + cbn in H1.
-          destruct (default_dvalue_of_dtyp t) eqn: HT. inv H1. inv H1.
-          pose proof DVALUE_Array_typ as ARR.
-          specialize (ARR (repeat d (Pos.to_nat p)) (N.to_nat (N.pos p)) t).
-          rewrite Nnat.N2Nat.id in ARR.
-          cbn in *.
-          apply ARR.
-          * apply forall_repeat_true.
-            apply IHt. reflexivity.
-          * apply repeat_length.
-      - revert H. induction fields.
-        + intros. inv H0. constructor.
-        + intros.
-          assert (forall u : dtyp,
-              In u fields ->
-              forall v : dvalue,
-                inr v = default_dvalue_of_dtyp u -> dvalue_has_dtyp v u).
-          { intros. apply H. apply in_cons. auto. auto. }
-          specialize (IHfields H1). clear H1.
-          Opaque map_monad.
-          (* Reduce H0 *)
-          cbn in H0.
-          rewrite list_cons_app in H0.
-          rewrite map_monad_app in H0. cbn in H0.
-          Transparent map_monad.
-          unfold map_monad at 1 in H0.
-          Opaque map_monad. cbn in H0.
-          destruct (default_dvalue_of_dtyp a) eqn: A_DEFAULT.
-          inv H0.
-          destruct (map_monad default_dvalue_of_dtyp fields) eqn: FIELDS.
-          inv H0.
-          inv H0. constructor. apply H. apply in_eq.
-          symmetry. auto.
-          apply IHfields. cbn. rewrite FIELDS. reflexivity.
-      - revert H. induction fields.
-        + intros. inv H0. constructor.
-        + intros.
-          assert (forall u : dtyp,
-              In u fields ->
-              forall v : dvalue,
-                inr v = default_dvalue_of_dtyp u -> dvalue_has_dtyp v u).
-          { intros. apply H. apply in_cons. auto. auto. }
-          specialize (IHfields H1). clear H1.
-          Opaque map_monad.
-          (* Reduce H0 *)
-          cbn in H0.
-          rewrite list_cons_app in H0.
-          rewrite map_monad_app in H0. cbn in H0.
-          Transparent map_monad.
-          unfold map_monad at 1 in H0.
-          Opaque map_monad. cbn in H0.
-          destruct (default_dvalue_of_dtyp a) eqn: A_DEFAULT.
-          inv H0.
-          destruct (map_monad default_dvalue_of_dtyp fields) eqn: FIELDS.
-          inv H0.
-          inv H0. constructor. apply H. apply in_eq.
-          symmetry. auto.
-          apply IHfields. cbn. rewrite FIELDS. reflexivity.
-      - intros. subst. inversion H. clear H.
-        revert H1. revert v. revert IHt. revert t.
-        induction sz.
-        + intros. cbn in H1.
-          pose proof DVALUE_Vector_typ.
-          specialize (H nil (N.to_nat 0)).
-          rewrite Nnat.N2Nat.id in H.
-          destruct t; inv H1;
-              try
-                (apply H;
-                 [constructor | constructor |
-                  unfold vector_dtyp; intuition]).
-          destruct (default_dvalue_of_dtyp_i sz) eqn: HI; inv H2.
-          apply H. constructor. auto. unfold vector_dtyp. left.
-          exists sz. reflexivity.
-        + intros. cbn in H1.
-          destruct t; inv H1;
-            try (
-                rewrite <- positive_nat_N;
-                   constructor; [apply forall_repeat_true ; constructor |
-                          apply repeat_length |
-                          unfold vector_dtyp ; intuition ]).
-          destruct (default_dvalue_of_dtyp_i sz) eqn: SZ; inv H0.
-            pose proof DVALUE_Vector_typ.
-            rewrite <- positive_nat_N. apply H.
-            apply forall_repeat_true. apply IHt. symmetry. auto.
-            apply repeat_length.
-            left. exists sz. reflexivity.
-    Qed.
 
    Transparent map_monad.
    Lemma concretize_u_concretize_uvalue : forall u, concretize_u u (concretize_uvalue u).
     Proof.
-      intros u.
-      induction u; try do_it.
-      - cbn. (* destruct (default_dvalue_of_dtyp t) eqn: EQ. *)
+      (* intros u. *)
+      (* induction u; try do_it. *)
+      (* - (* cbn. *) (* destruct (default_dvalue_of_dtyp t) eqn: EQ. *) *)
     (*     econstructor. Unshelve. 3 : { exact DVALUE_None. } *)
     (*     intro. inv H. *)
     (*     apply Concretize_Undef. apply dvalue_default. symmetry. auto. *)
