src/coq/Transformations/UndefRefinementFacts.v
@@ -16,10 +16,19 @@ From Vellvm Require Import
      PropT
      Syntax.Traversal.
 
+From Vellvm.Semantics Require Import
+     Memory.Sizeof
+     Memory.MemBytes
+     GepM.
+
+From Vellvm.Utils Require Import
+     Tactics.
+
 From Vellvm.Handlers Require Import
      Stack
      Local
-     Global.
+     Global
+     Serialization.
 
 From ITree Require Import
      ITree
@@ -45,287 +54,432 @@ Import Monads.
 Require Import Morphisms.
 Require Import Relations.
 
-Import R.
-Import TopLevelEnv.
-Import IO.
-Import D.
+(* Import R. *)
+(* Import TopLevelEnv. *)
+(* Import IO. *)
+(* Import D. *)
+
+Import MemoryAddress.
 
 
-(* -------------------------------------------------------- *)
-(* Facts about multiplication and undef                     *)
-(* -------------------------------------------------------- *)
+Module Make (A:MemoryAddress.ADDRESS)(SIZE:Sizeof)(LLVMEvents: LLVM_INTERACTIONS(A)(SIZE))(PTOI:PTOI(A))(PROV:PROVENANCE(A))(ITOP:ITOP(A)(PROV))(GEP:GEPM(A)(SIZE)(LLVMEvents))(BYTE_IMPL:ByteImpl(A)(SIZE)(LLVMEvents)).
 
-Theorem undef_refines_mul_undef_undef:
-  refine_uvalue (UVALUE_Undef (DTYPE_I 64)) (UVALUE_IBinop (Mul false false) (UVALUE_Undef (DTYPE_I 64)) (UVALUE_Undef (DTYPE_I 64))).
-Proof.
-  constructor.
-  intros dv H.
-  apply Concretize_IBinop with (dv1:=DVALUE_I64 one) (dv2:=dv).
-  - apply Concretize_Undef. constructor.
-  - auto.
-  - simpl. inversion H; subst.
-    + inversion H0.
-    + inversion H1; subst; auto.
-      unfold DynamicValues.Int64.mul. unfold DynamicValues.Int64.one.
-      replace (DynamicValues.Int64.unsigned (DynamicValues.Int64.repr 1) *
-               DynamicValues.Int64.unsigned x) with (DynamicValues.Int64.unsigned x).
-      * destruct (Eqv.eqv_dec_p 64%nat 1%nat); rewrite DynamicValues.Int64.repr_unsigned; reflexivity.
-      * rewrite Integers.Int64.unsigned_repr; try lia; cbn; try omega.
-Qed.
+  Module Conc := Serialization.Make A SIZE LLVMEvents PTOI PROV ITOP GEP BYTE_IMPL.
 
-Lemma rel_prime_mod_mul :
-  forall a b x,
-    Znumtheory.rel_prime a b ->
-  exists k, (a * k) mod b = x.
-Proof.
-Admitted.
+  Module Ref := Refinement.Make A SIZE LLVMEvents PTOI PROV ITOP GEP BYTE_IMPL.
+  Import Ref.
+  Import LLVMEvents.
+  Import Conc.
 
-Lemma mod_range :
-  forall x m, -1 < x mod m < m.
-Proof.
-Admitted.
+  (* -------------------------------------------------------- *)
+  (* Facts about multiplication and undef                     *)
+  (* -------------------------------------------------------- *)
 
-Lemma Int64_mul_mod :
-  forall a b intrange,
-    (DynamicValues.Int64.mul (DynamicValues.Int64.repr a)
-                             (DynamicValues.Int64.repr b)) = 
-    {| DynamicValues.Int64.intval := ((a * b) mod DynamicValues.Int64.modulus);
-       DynamicValues.Int64.intrange := intrange
-    |}.
-Proof.
-Admitted.
+  Instance proper_refine_uvalue_ibinop {op v2 rv} : Proper ((fun x y => refine_uvalue y x) ==> (fun (x y : Prop) => x -> y)) (fun v1 => refine_uvalue (UVALUE_IBinop op v1 v2) rv).
+  Proof.    
+    unfold Proper, respectful.
+    intros x y Ryx Ribop.
+    constructor.
+    - intros CONTRA. subst.
+      apply refine_poison in Ribop. inversion Ribop.
+    - intros dv0 Conc.
+      inversion Ribop; subst.
+      pose proof (H0 dv0 Conc).
 
-Theorem undef_refines_mul_undef_relprime :
-  forall a,
-    Znumtheory.rel_prime a DynamicValues.Int64.modulus -> 
-    refine_uvalue (UVALUE_Undef (DTYPE_I 64))
-                  (UVALUE_IBinop (Mul false false)
-                                 (UVALUE_Undef (DTYPE_I 64)) (UVALUE_I64 (DynamicValues.Int64.repr a))).
-Proof.
-  intros a Hrp.
-  constructor.
-  intros dv H.
-  inversion H; subst.
-  - inversion H0. 
-  - inversion H1; subst; inversion H; subst.
-    + inversion H0.
-    + destruct x eqn:Hx.
-      pose proof rel_prime_mod_mul a DynamicValues.Int64.modulus intval Hrp as Hmod.
+      inversion Ryx; subst.
+      + (* x could be a refinement of poison
 
-      destruct Hmod as [k Hmod].
-      rewrite Z.mul_comm in Hmod.
+           refine_uvalue has an UndefPoison case which means anything
+           refines poison.
+         *)
+        (* In this case, eval_iop should return poison,
 
-      match goal with
-      | [ H : concretize (UVALUE_Undef ?t) ?dv |- concretize (UVALUE_IBinop _ (UVALUE_Undef ?t) (UVALUE_I64 ?v1)) ?dv ]
-        => apply Concretize_IBinop with (dv2:=(DVALUE_I64 v1)) (dv1:=DVALUE_I64 (repr k))
-      end.
-   -- apply Concretize_Undef; constructor.
-   -- constructor; reflexivity.
-   -- subst; simpl.
-      destruct (Eqv.eqv_dec_p 64%nat 1%nat);
-        (rewrite (Int64_mul_mod k a intrange); reflexivity).
-Qed.
-
-Theorem undef_refines_mul_relprime_undef :
-  forall a,
-    Znumtheory.rel_prime a DynamicValues.Int64.modulus -> 
-    refine_uvalue (UVALUE_Undef (DTYPE_I 64))
-                  (UVALUE_IBinop (Mul false false)
-                                 (UVALUE_I64 (DynamicValues.Int64.repr a)) (UVALUE_Undef (DTYPE_I 64))).
-Proof.
-  intros a Hrp.
-  constructor.
-  intros dv H.
-  inversion H; subst.
-  - inversion H0. 
-  - inversion H1; subst; inversion H; subst.
-    + inversion H0.
-    + destruct x eqn:Hx.
-      pose proof rel_prime_mod_mul a DynamicValues.Int64.modulus intval Hrp as Hmod.
-
-      destruct Hmod as [k Hmod].
-
-    match goal with
-    | [ H : concretize (UVALUE_Undef ?t) ?dv |- concretize (UVALUE_IBinop _ (UVALUE_I64 ?v1) (UVALUE_Undef ?t)) ?dv ]
-      => apply Concretize_IBinop with (dv1:=(DVALUE_I64 v1)) (dv2:=DVALUE_I64 (repr k))
-    end.
-   -- constructor; reflexivity.
-   -- apply Concretize_Undef; constructor.
-   -- subst; simpl.
-      destruct (Eqv.eqv_dec_p 64%nat 1%nat);
-        (rewrite (Int64_mul_mod a k intrange); reflexivity).
-Qed.
-
-Lemma zero_refines_undef :
-  refine_uvalue (UVALUE_I64 (DynamicValues.Int64.repr 0)) (UVALUE_Undef (DTYPE_I 64)).
-Proof.
-  constructor. intros dv H.
-  inversion H; subst.
-  inversion H0; subst.
-  apply Concretize_Undef.
-  constructor.
-Qed.
-
-Lemma zero_refines_undef_mul_a :
-  forall a,
-    refine_uvalue (UVALUE_I64 (DynamicValues.Int64.repr 0))
-                  (UVALUE_IBinop (Mul false false)
-                                 (UVALUE_Undef (DTYPE_I 64)) (UVALUE_I64 a)).
-Proof.
-  constructor. intros dv H.
-  inversion H; subst.
-  inversion H0; subst.
-  simpl in *.
-  clear H0.
-
-  eapply Concretize_IBinop with
-      (dv1:=DVALUE_I64 (DynamicValues.Int64.repr 0)).
-
-  apply Concretize_Undef.
-  constructor.
-  constructor. reflexivity.
-Admitted.
-
-
-Lemma zero_refines_a_mul_undef :
-  forall a,
-    refine_uvalue (UVALUE_I64 (DynamicValues.Int64.repr 0))
-                  (UVALUE_IBinop (Mul false false)
-                                 (UVALUE_I64 a) (UVALUE_Undef (DTYPE_I 64))).
-Proof.
-Admitted.
-
-
-(* -------------------------------------------------------- *)
-(* Facts about undef and bitwise and                        *)
-(* -------------------------------------------------------- *)
-
-Theorem undef_refines_and_undef_undef:
-  refine_uvalue (UVALUE_Undef (DTYPE_I 64)) (UVALUE_IBinop And (UVALUE_Undef (DTYPE_I 64)) (UVALUE_Undef (DTYPE_I 64))).
-Proof.
-  constructor.
-  intros dv H.
-  apply Concretize_IBinop with (dv1:=DVALUE_I64 (DynamicValues.Int64.repr (Z.ones 64))) (dv2:=dv).
-  - apply Concretize_Undef. constructor.
-  - auto.
-  - simpl. inversion H; subst.
-    + inversion H0.
-    + inversion H1; subst; auto.
-      unfold DynamicValues.Int64.and.
-      replace (Z.land
-                 (DynamicValues.Int64.unsigned
-                    (DynamicValues.Int64.repr (Z.ones 64)))
-                 (DynamicValues.Int64.unsigned x))
-        with (DynamicValues.Int64.unsigned x).
-      * destruct (Eqv.eqv_dec_p 64%nat 1%nat); rewrite DynamicValues.Int64.repr_unsigned; reflexivity.
-      * rewrite Integers.Int64.unsigned_repr by (cbn; lia).
-        rewrite Z.land_comm.
-        rewrite Z.land_ones by lia.
-        rewrite Z.mod_small. reflexivity.
-        
+           
+         *)
+      
+      inversion Ryx; subst.
+      + red. red.
+        rewrite concretize_uvalueM_equation.
         cbn.
-        pose proof DynamicValues.Int64.unsigned_range_2 x.
-        cbn in H0.
-        lia.
-Qed.
-
-(* -------------------------------------------------------- *)
-(* Facts about undef and bitwise or                         *)
-(* -------------------------------------------------------- *)
-
-Theorem undef_refines_or_undef_undef:
-  refine_uvalue (UVALUE_Undef (DTYPE_I 64)) (UVALUE_IBinop Or (UVALUE_Undef (DTYPE_I 64)) (UVALUE_Undef (DTYPE_I 64))).
-Proof.
-  constructor.
-  intros dv H.
-  apply Concretize_IBinop with (dv1:=DVALUE_I64 (DynamicValues.Int64.repr 0)) (dv2:=dv).
-  - apply Concretize_Undef. constructor.
-  - auto.
-  - simpl. inversion H; subst.
-    + inversion H0.
-    + inversion H1; subst; auto.
-      unfold DynamicValues.Int64.or.
-      replace (Z.lor
-                 (DynamicValues.Int64.unsigned
-                    (DynamicValues.Int64.repr 0))
-                 (DynamicValues.Int64.unsigned x))
-        with (DynamicValues.Int64.unsigned x).
-      * destruct (Eqv.eqv_dec_p 64%nat 1%nat); rewrite DynamicValues.Int64.repr_unsigned; reflexivity.
-      * rewrite Integers.Int64.unsigned_repr by (cbn; lia).
+        unfold bind_MPropT.
+        eexists. exists (fun _ => ret dv0).
+        split; [reflexivity|].
+        split; [reflexivity|].
+        intros a MReta.
+        inversion MReta; subst.
+        cbn.
+        exists (ret dv0). exists ret.
+        split.
+        admit.
+        split.
+        cbn.
         reflexivity.
-Qed.
+        intros a0 H2.
+        inversion H2;  subst.
+        cbn.
+        destruct a0.
+        cbn.
+        inversion MReta; subst.
+        cbn.
 
 
-(* -------------------------------------------------- *)
-(* Division and undef facts                           *)
-(* -------------------------------------------------- *)
+        { destruct v2.
 
-Theorem undef_refines_undef_udiv_1:
+
+          rewrite concretize_uvalueM_equation.
+          cbn.
+
+            rewrite c
+
+        }
+
+        [reflexivity|].
+        split; [reflexivity|].
+        
+        admit.
+        admit.
+      + admit.
+
+
+
+    constructor; [intros CONTRA; inversion CONTRA|].
+    intros dv H.
+
+    clear H. exfalso. clear dv.
+
+    (*   eapply Concretize_IBinop. *)
+    (* } *)
+    
+    (* eapply Concretize_IBinop. with (dv1:=DVALUE_I64 one) (dv2:=dv). *)
+    (* - apply Concretize_Undef. constructor. *)
+    (* - auto. *)
+    (* - simpl. inversion H; subst. *)
+    (*   + inversion H0. *)
+    (*   + inversion H1; subst; auto. *)
+    (*     unfold DynamicValues.Int64.mul. unfold DynamicValues.Int64.one. *)
+    (*     replace (DynamicValues.Int64.unsigned (DynamicValues.Int64.repr 1) * *)
+    (*              DynamicValues.Int64.unsigned x) with (DynamicValues.Int64.unsigned x). *)
+    (*     * destruct (Eqv.eqv_dec_p 64%nat 1%nat); rewrite DynamicValues.Int64.repr_unsigned; reflexivity. *)
+    (*     * rewrite Integers.Int64.unsigned_repr; try lia; cbn; try omega. *)
+
+  Admitted.
+
+  Theorem undef_refines_mul_1_undef :
+    refine_uvalue
+      (UVALUE_IBinop (Mul false false) (UVALUE_I64 one)
+                     (UVALUE_Undef (DTYPE_I 64))) (UVALUE_Undef (DTYPE_I 64)).
+  Proof.
+    constructor.
+    intros CONTRA; inversion CONTRA.
+
+    intros dv H.
+    rewrite concretize_equation in *.
+    red in H; red.
+    cbn in H.
+
+    cbn.
+
+    unfold bind_MPropT.
+    eexists. exists (fun x => ret dv).
+    split.
+    - reflexivity.
+    - split.
+      + cbn. reflexivity.
+      + intros a MRet.
+        exists {| EitherMonad.unEitherT := inr (inr dv) |}. exists ret.
+        split; auto.
+        split; [cbn; reflexivity|].
+
+        intros dv' MRetdv.
+        inversion MRet.
+        inversion MRetdv.
+        subst.
+
+        inversion H; subst.
+        cbn.
+
+        break_inner_match.
+        rewrite DynamicValues.Int64.mul_commut.
+        rewrite DynamicValues.Int64.mul_one.
+        reflexivity.
+
+        rewrite DynamicValues.Int64.mul_commut.
+        rewrite DynamicValues.Int64.mul_one.
+        reflexivity.
+  Qed.
+
+  Theorem undef_refines_mul_undef_undef:
+    refine_uvalue (UVALUE_IBinop (Mul false false) (UVALUE_Undef (DTYPE_I 64)) (UVALUE_Undef (DTYPE_I 64))) (UVALUE_Undef (DTYPE_I 64)).
+  Proof.
+    assert (refine_uvalue (UVALUE_Undef (DTYPE_I 64)) (UVALUE_I64 one)).
+    { constructor; intuition.
+      inversion H.
+      rewrite concretize_equation in *.
+      red in H.
+      red.
+      cbn in *.
+
+      inversion H.
+      constructor.
+    }
+
+    eapply proper_refine_uvalue_ibinop; eauto.
+    apply undef_refines_mul_1_undef.
+  Qed.
+
+  Lemma rel_prime_mod_mul :
+    forall a b x,
+      Znumtheory.rel_prime a b ->
+      exists k, (a * k) mod b = x.
+  Proof.
+  Admitted.
+
+  Lemma mod_range :
+    forall x m, -1 < x mod m < m.
+  Proof.
+  Admitted.
+
+  Lemma Int64_mul_mod :
+    forall a b intrange,
+      (DynamicValues.Int64.mul (DynamicValues.Int64.repr a)
+                               (DynamicValues.Int64.repr b)) = 
+      {| DynamicValues.Int64.intval := ((a * b) mod DynamicValues.Int64.modulus);
+         DynamicValues.Int64.intrange := intrange
+      |}.
+  Proof.
+  Admitted.
+
+  Theorem undef_refines_mul_undef_relprime :
+    forall a,
+      Znumtheory.rel_prime a DynamicValues.Int64.modulus -> 
+      refine_uvalue (UVALUE_Undef (DTYPE_I 64))
+                    (UVALUE_IBinop (Mul false false)
+                                   (UVALUE_Undef (DTYPE_I 64)) (UVALUE_I64 (DynamicValues.Int64.repr a))).
+  Proof.
+    intros a Hrp.
+    constructor.
+    intros dv H.
+    inversion H; subst.
+    - inversion H0. 
+    - inversion H1; subst; inversion H; subst.
+      + inversion H0.
+      + destruct x eqn:Hx.
+        pose proof rel_prime_mod_mul a DynamicValues.Int64.modulus intval Hrp as Hmod.
+
+        destruct Hmod as [k Hmod].
+        rewrite Z.mul_comm in Hmod.
+
+        match goal with
+        | [ H : concretize (UVALUE_Undef ?t) ?dv |- concretize (UVALUE_IBinop _ (UVALUE_Undef ?t) (UVALUE_I64 ?v1)) ?dv ]
+          => apply Concretize_IBinop with (dv2:=(DVALUE_I64 v1)) (dv1:=DVALUE_I64 (repr k))
+        end.
+        -- apply Concretize_Undef; constructor.
+        -- constructor; reflexivity.
+        -- subst; simpl.
+           destruct (Eqv.eqv_dec_p 64%nat 1%nat);
+             (rewrite (Int64_mul_mod k a intrange); reflexivity).
+  Qed.
+
+  Theorem undef_refines_mul_relprime_undef :
+    forall a,
+      Znumtheory.rel_prime a DynamicValues.Int64.modulus -> 
+      refine_uvalue (UVALUE_Undef (DTYPE_I 64))
+                    (UVALUE_IBinop (Mul false false)
+                                   (UVALUE_I64 (DynamicValues.Int64.repr a)) (UVALUE_Undef (DTYPE_I 64))).
+  Proof.
+    intros a Hrp.
+    constructor.
+    intros dv H.
+    inversion H; subst.
+    - inversion H0. 
+    - inversion H1; subst; inversion H; subst.
+      + inversion H0.
+      + destruct x eqn:Hx.
+        pose proof rel_prime_mod_mul a DynamicValues.Int64.modulus intval Hrp as Hmod.
+
+        destruct Hmod as [k Hmod].
+
+        match goal with
+        | [ H : concretize (UVALUE_Undef ?t) ?dv |- concretize (UVALUE_IBinop _ (UVALUE_I64 ?v1) (UVALUE_Undef ?t)) ?dv ]
+          => apply Concretize_IBinop with (dv1:=(DVALUE_I64 v1)) (dv2:=DVALUE_I64 (repr k))
+        end.
+        -- constructor; reflexivity.
+        -- apply Concretize_Undef; constructor.
+        -- subst; simpl.
+           destruct (Eqv.eqv_dec_p 64%nat 1%nat);
+             (rewrite (Int64_mul_mod a k intrange); reflexivity).
+  Qed.
+
+  Lemma zero_refines_undef :
+    refine_uvalue (UVALUE_I64 (DynamicValues.Int64.repr 0)) (UVALUE_Undef (DTYPE_I 64)).
+  Proof.
+    constructor. intros dv H.
+    inversion H; subst.
+    inversion H0; subst.
+    apply Concretize_Undef.
+    constructor.
+  Qed.
+
+  Lemma zero_refines_undef_mul_a :
+    forall a,
+      refine_uvalue (UVALUE_I64 (DynamicValues.Int64.repr 0))
+                    (UVALUE_IBinop (Mul false false)
+                                   (UVALUE_Undef (DTYPE_I 64)) (UVALUE_I64 a)).
+  Proof.
+    constructor. intros dv H.
+    inversion H; subst.
+    inversion H0; subst.
+    simpl in *.
+    clear H0.
+
+    eapply Concretize_IBinop with
+        (dv1:=DVALUE_I64 (DynamicValues.Int64.repr 0)).
+
+    apply Concretize_Undef.
+    constructor.
+    constructor. reflexivity.
+  Admitted.
+
+
+  Lemma zero_refines_a_mul_undef :
+    forall a,
+      refine_uvalue (UVALUE_I64 (DynamicValues.Int64.repr 0))
+                    (UVALUE_IBinop (Mul false false)
+                                   (UVALUE_I64 a) (UVALUE_Undef (DTYPE_I 64))).
+  Proof.
+  Admitted.
+
+
+  (* -------------------------------------------------------- *)
+  (* Facts about undef and bitwise and                        *)
+  (* -------------------------------------------------------- *)
+
+  Theorem undef_refines_and_undef_undef:
+    refine_uvalue (UVALUE_Undef (DTYPE_I 64)) (UVALUE_IBinop And (UVALUE_Undef (DTYPE_I 64)) (UVALUE_Undef (DTYPE_I 64))).
+  Proof.
+    constructor.
+    intros dv H.
+    apply Concretize_IBinop with (dv1:=DVALUE_I64 (DynamicValues.Int64.repr (Z.ones 64))) (dv2:=dv).
+    - apply Concretize_Undef. constructor.
+    - auto.
+    - simpl. inversion H; subst.
+      + inversion H0.
+      + inversion H1; subst; auto.
+        unfold DynamicValues.Int64.and.
+        replace (Z.land
+                   (DynamicValues.Int64.unsigned
+                      (DynamicValues.Int64.repr (Z.ones 64)))
+                   (DynamicValues.Int64.unsigned x))
+          with (DynamicValues.Int64.unsigned x).
+        * destruct (Eqv.eqv_dec_p 64%nat 1%nat); rewrite DynamicValues.Int64.repr_unsigned; reflexivity.
+        * rewrite Integers.Int64.unsigned_repr by (cbn; lia).
+          rewrite Z.land_comm.
+          rewrite Z.land_ones by lia.
+          rewrite Z.mod_small. reflexivity.
+          
+          cbn.
+          pose proof DynamicValues.Int64.unsigned_range_2 x.
+          cbn in H0.
+          lia.
+  Qed.
+
+  (* -------------------------------------------------------- *)
+  (* Facts about undef and bitwise or                         *)
+  (* -------------------------------------------------------- *)
+
+  Theorem undef_refines_or_undef_undef:
+    refine_uvalue (UVALUE_Undef (DTYPE_I 64)) (UVALUE_IBinop Or (UVALUE_Undef (DTYPE_I 64)) (UVALUE_Undef (DTYPE_I 64))).
+  Proof.
+    constructor.
+    intros dv H.
+    apply Concretize_IBinop with (dv1:=DVALUE_I64 (DynamicValues.Int64.repr 0)) (dv2:=dv).
+    - apply Concretize_Undef. constructor.
+    - auto.
+    - simpl. inversion H; subst.
+      + inversion H0.
+      + inversion H1; subst; auto.
+        unfold DynamicValues.Int64.or.
+        replace (Z.lor
+                   (DynamicValues.Int64.unsigned
+                      (DynamicValues.Int64.repr 0))
+                   (DynamicValues.Int64.unsigned x))
+          with (DynamicValues.Int64.unsigned x).
+        * destruct (Eqv.eqv_dec_p 64%nat 1%nat); rewrite DynamicValues.Int64.repr_unsigned; reflexivity.
+        * rewrite Integers.Int64.unsigned_repr by (cbn; lia).
+          reflexivity.
+  Qed.
+
+
+  (* -------------------------------------------------- *)
+  (* Division and undef facts                           *)
+  (* -------------------------------------------------- *)
+
+  Theorem undef_refines_undef_udiv_1:
     refine_uvalue (UVALUE_Undef (DTYPE_I 64)) (UVALUE_IBinop (UDiv false) (UVALUE_Undef (DTYPE_I 64)) (UVALUE_I64 (DynamicValues.Int64.repr 1))).
-Proof.
-  constructor.
-  intros dv H.
-  apply Concretize_IBinop with (dv1:=dv) (dv2:=DVALUE_I64 (DynamicValues.Int64.repr 1)).
-  - auto.
-  - constructor; reflexivity.
-  - inversion H; subst; simpl in *.
-    + inversion H0.
-    + inversion H1. simpl.
-      destruct (DynamicValues.Int64.unsigned (DynamicValues.Int64.repr 1) =?
-                0)%Z eqn:Heq.
-      inversion Heq.
-      simpl.
-      rewrite DynamicValues.Int64.divu_one.
-      reflexivity.
-Qed.
+  Proof.
+    constructor.
+    intros dv H.
+    apply Concretize_IBinop with (dv1:=dv) (dv2:=DVALUE_I64 (DynamicValues.Int64.repr 1)).
+    - auto.
+    - constructor; reflexivity.
+    - inversion H; subst; simpl in *.
+      + inversion H0.
+      + inversion H1. simpl.
+        destruct (DynamicValues.Int64.unsigned (DynamicValues.Int64.repr 1) =?
+                  0)%Z eqn:Heq.
+        inversion Heq.
+        simpl.
+        rewrite DynamicValues.Int64.divu_one.
+        reflexivity.
+  Qed.
 
-Theorem undef_refines_undef_sdiv_1:
+  Theorem undef_refines_undef_sdiv_1:
     refine_uvalue (UVALUE_Undef (DTYPE_I 64)) (UVALUE_IBinop (SDiv false) (UVALUE_Undef (DTYPE_I 64)) (UVALUE_I64 (DynamicValues.Int64.repr 1))).
-Proof.
-  constructor.
-  intros dv H.
-  apply Concretize_IBinop with (dv1:=dv) (dv2:=DVALUE_I64 (DynamicValues.Int64.repr 1)).
-  - auto.
-  - constructor; reflexivity.
-  - inversion H; subst; simpl in *.
-    + inversion H0.
-    + inversion H1. simpl.
-      destruct (DynamicValues.Int64.signed (DynamicValues.Int64.repr 1) =?
-                0)%Z eqn:Heq.
-      inversion Heq.
-      simpl.
-      rewrite DynamicValues.Int64.divs_one.
-      reflexivity.
-      cbn.
-      lia.
-Qed.
+  Proof.
+    constructor.
+    intros dv H.
+    apply Concretize_IBinop with (dv1:=dv) (dv2:=DVALUE_I64 (DynamicValues.Int64.repr 1)).
+    - auto.
+    - constructor; reflexivity.
+    - inversion H; subst; simpl in *.
+      + inversion H0.
+      + inversion H1. simpl.
+        destruct (DynamicValues.Int64.signed (DynamicValues.Int64.repr 1) =?
+                  0)%Z eqn:Heq.
+        inversion Heq.
+        simpl.
+        rewrite DynamicValues.Int64.divs_one.
+        reflexivity.
+        cbn.
+        lia.
+  Qed.
 
-Theorem zero_refines_undef_urem_1:
+  Theorem zero_refines_undef_urem_1:
     refine_uvalue (UVALUE_I64 (DynamicValues.Int64.repr 0)) (UVALUE_IBinop URem (UVALUE_Undef (DTYPE_I 64)) (UVALUE_I64 (DynamicValues.Int64.repr 1))).
-Proof.
-  constructor.
-  intros dv H. inversion H; subst; inversion H0; subst.
-  apply Concretize_IBinop with (dv1:=DVALUE_I64 (DynamicValues.Int64.repr 0)) (dv2:=DVALUE_I64 (DynamicValues.Int64.repr 1)).
-  - apply Concretize_Undef. constructor.
-  - constructor. reflexivity.
-  - simpl.
-    destruct (DynamicValues.Int64.unsigned (DynamicValues.Int64.repr 1) =?
-              0)%Z eqn:Heq; simpl.
-    inversion Heq.
+  Proof.
+    constructor.
+    intros dv H. inversion H; subst; inversion H0; subst.
+    apply Concretize_IBinop with (dv1:=DVALUE_I64 (DynamicValues.Int64.repr 0)) (dv2:=DVALUE_I64 (DynamicValues.Int64.repr 1)).
+    - apply Concretize_Undef. constructor.
+    - constructor. reflexivity.
+    - simpl.
+      destruct (DynamicValues.Int64.unsigned (DynamicValues.Int64.repr 1) =?
+                0)%Z eqn:Heq; simpl.
+      inversion Heq.
 
-    rewrite Integers.Int64.modu_one. reflexivity.
-Qed.
+      rewrite Integers.Int64.modu_one. reflexivity.
+  Qed.
 
-Theorem zero_refines_undef_srem_1:
+  Theorem zero_refines_undef_srem_1:
     refine_uvalue (UVALUE_I64 (DynamicValues.Int64.repr 0)) (UVALUE_IBinop SRem (UVALUE_Undef (DTYPE_I 64)) (UVALUE_I64 (DynamicValues.Int64.repr 1))).
-Proof.
-  constructor.
-  intros dv H. inversion H; subst; inversion H0; subst.
-  apply Concretize_IBinop with (dv1:=DVALUE_I64 (DynamicValues.Int64.repr 0)) (dv2:=DVALUE_I64 (DynamicValues.Int64.repr 1)).
-  - apply Concretize_Undef. constructor.
-  - constructor. reflexivity.
-  - simpl.
-    destruct (DynamicValues.Int64.signed (DynamicValues.Int64.repr 1) =?
-              0)%Z eqn:Heq; simpl.
-    inversion Heq.
-Admitted.
+  Proof.
+    constructor.
+    intros dv H. inversion H; subst; inversion H0; subst.
+    apply Concretize_IBinop with (dv1:=DVALUE_I64 (DynamicValues.Int64.repr 0)) (dv2:=DVALUE_I64 (DynamicValues.Int64.repr 1)).
+    - apply Concretize_Undef. constructor.
+    - constructor. reflexivity.
+    - simpl.
+      destruct (DynamicValues.Int64.signed (DynamicValues.Int64.repr 1) =?
+                0)%Z eqn:Heq; simpl.
+      inversion Heq.
+  Admitted.
